cast_sub/subtyping.v
@@ -3,9 +3,14 @@
 *)
 Require Import Metalib.Metatheory.
 Require Import Program.Equality.
-Require Import subtyping.AmberBase.
+Require Import subtyping.AmberLocal.
+(* Require Import subtyping.Decidability. *)
 Require Export rules_inf.
+Require Export LibTactics.
+Require Import Lia.
 
+
+(* Relating our types to TOPLAS types *)
 
 Fixpoint trans_ty (A : typ) : Rules.typ :=
   match A with
@@ -29,22 +34,202 @@ Fixpoint back_ty (A : Rules.typ) : typ :=
   | typ_mu A => t_mu (back_ty A)
   end.
 
-Lemma AmberWF_to_Isowfe: forall AE,
-  AmberWF AE -> wfe_amber AE.
+Lemma AmberdomA_IsodomA: forall AE,
+  domA AE [=] AmberBase.domA AE.
 Proof.
   intros.
+  induction AE; simpl; eauto.
+  - reflexivity.
+  - destruct a. fsetdec.
+Qed.
+  
+
+Lemma AmberWF_Isowfe: forall AE,
+  AmberWF AE <-> wfe_amber AE.
+Proof with auto.
+  intros. split;intro.
+  + induction H; simpl; eauto.
+  + induction H; simpl; eauto.
+Qed.
+
+
+#[export]
+Hint Extern 1 (AmberWF ?AE) =>
+  match goal with
+  | H: wfe_amber AE |- _ => apply AmberWF_Isowfe in H
+  end : core.
+
+#[export]
+Hint Extern 1 (wfe_amber ?AE) =>
+  match goal with
+  | H: AmberWF AE |- _ => apply AmberWF_Isowfe in H
+  end : core.
+
+Lemma trans_ty_open_typ_wrt_typ: forall A X, degree_typ_wrt_typ 1 A ->
+  trans_ty (open_typ_wrt_typ A (t_var_f X)) = open_tt (trans_ty A) X.
+Proof with auto.
+  intros. unfold open_typ_wrt_typ.
+  unfold open_tt.
+  revert H.
+  generalize 0. intros.
+  inductions H;intros...
+  - 
+    simpl. destruct (lt_eq_lt_dec n2 n) as [[?|?]|?].
+    + simpl. destruct (n == n2);try lia...
+    + subst. simpl. destruct (n == n);try lia...
+    + simpl. destruct (n == n2);try lia...
+  - simpl. rewrite IHdegree_typ_wrt_typ1... 
+    rewrite IHdegree_typ_wrt_typ2...
+  - simpl. f_equal.
+    rewrite IHdegree_typ_wrt_typ...
+Qed.
+
+Lemma trans_back_ty: forall A,
+  trans_ty (back_ty A) = A.
+Proof with auto.
+  inductions A;simpl...
+  - rewrite IHA...
+  - rewrite IHA1;rewrite IHA2...
+Qed.
+
+Lemma back_trans_ty: forall A,
+  back_ty (trans_ty A) = A.
+Proof with auto.
+  inductions A;simpl...
+  - rewrite IHA1;rewrite IHA2...
+  - rewrite IHA...
+Qed.
+
+
+
+Lemma back_ty_open_tt: forall A (X:atom),
+  WFC A 1 ->
+  back_ty (open_tt A X) = open_typ_wrt_typ (back_ty A) (t_var_f X).
+Proof with auto.
+  intros. 
+  unfold open_typ_wrt_typ.
+  unfold open_tt.
+  revert H.
+  generalize 0. intros.
+  inductions H;intros...
+  - 
+    simpl. destruct (lt_eq_lt_dec b n) as [[?|?]|?].
+    + simpl. destruct (n == b);try lia...
+    + subst. simpl. destruct (n == n);try lia...
+    + simpl. destruct (n == b);try lia...
+  - simpl. rewrite IHWFC1... 
+    rewrite IHWFC2...
+  - simpl. f_equal.
+    rewrite IHWFC...
+Qed.
+
+
+(* Lemma back_ty_open_tt: forall A (X:atom),
+  degree_typ_wrt_typ 1 (back_ty A) ->
+  back_ty (open_tt A X) = open_typ_wrt_typ (back_ty A) (t_var_f X).
+Proof with auto.
+  intros. 
+  forwards: trans_ty_open_typ_wrt_typ X H.
+  rewrite trans_back_ty in H0.
+  rewrite <- H0.
+  rewrite back_trans_ty...
+Qed. *)
+
+Lemma AmberWFT_lc: forall AE A,
+  AmberWFT AE A -> lc_typ A.
+Proof with auto.
+  intros.
   induction H; simpl; eauto.
-  - constructor...
-Admitted.
+  - pick_fresh X.
+    specialize_x_and_L X L.
+    pick_fresh Y'.
+    specialize_x_and_L Y' (L \u {{X}}).
+    apply lc_t_mu_exists with (X1:=X)...
+Qed.
+
+
+Lemma AmberWFT_Isowft: forall AE A,
+  AmberWFT AE A -> wf_amber AE (trans_ty A).
+Proof with auto.
+  intros.
+  induction H; simpl; eauto.
+  - apply wfa_rec with (L:=L).
+    intros. specialize (H _ H1). specialize (H0 _ H1).
+    specialize (H _ H2). specialize (H0 _ H2).
+    rewrite <- trans_ty_open_typ_wrt_typ...
+    { apply AmberWFT_lc in H. apply degree_typ_wrt_typ_of_lc_typ  in H.
+      apply degree_typ_wrt_typ_open_typ_wrt_typ_inv in H... }
+Qed.
+
+Lemma type_rename_env_aux: forall E A n,
+  WFC (rename_env E A) n -> WFC A n.
+Proof with auto.
+  intros.
+  inductions A...
+  - rewrite rename_bvar in H...
+  - rewrite rename_mu in H...
+    constructor. apply IHA.
+    inversion H...
+  - rewrite rename_arrow in H.
+    inversion H;subst...
+Qed.
+
+Lemma type_rename_env: forall E A,
+  type (rename_env E A) -> type A.
+Proof with auto.
+  intros.
+  apply close_type_wfc in H.
+  apply type_rename_env_aux in H.
+  inductions E...
+  - simpl in H. apply type_wfc_close...
+Qed.
+
+
+
+
+Lemma Isowft_AmberWFT: forall AE A,
+  wf_amber AE A -> AmberWFT AE (back_ty A).
+Proof with auto.
+  intros.
+  induction H; simpl; eauto.
+  - pick_fresh Y0. 
+    apply AWFT_rec with (L:=L \u fv_tt A \u AmberBase.domA E). { apply Y0. }
+    intros. rewrite <- back_ty_open_tt. { apply H0... }
+    { 
+      (* apply type_open_tt_WFC with (X:=X)... *)
+      specialize (H X Y).
+      apply wf_amber_to_WF in H...
+      simpl in H. rewrite <- subst_tt_fresh in H.
+      2:{ apply notin_fv_domA... apply notin_fv_tt_open_aux... }
+      apply soundness_wfa in H.
+      apply wfs_type in H.
+      apply type_rename_env in H.
+      apply type_open_tt_WFC in H...
+    }
+Qed.
+
+#[export]
+Hint Extern 1 (AmberWFT ?AE (back_ty ?A)) =>
+  match goal with
+  | H: wf_amber AE A |- _ => apply Isowft_AmberWFT in H
+  end : core.
+
+#[export]
+Hint Extern 1 (wf_amber ?AE (trans_ty ?A)) =>
+  match goal with
+  | H: AmberWFT AE A |- _ => apply AmberWFT_Isowft in H
+  end : core.
+
 
 
 Lemma AmberSubtyping_to_IsoSubtyping: forall G A B,
   AmberSubtyping G A B -> AmberBase.sub_amber G (trans_ty A) (trans_ty B).
-Proof.
+Proof with auto.
   intros.
   induction H; simpl; eauto.
-  - apply sam_nat...
+  - 
 Admitted.
+
 
 Theorem unfolding_lemma: forall A B,
   AmberSubtyping nil (t_mu A) (t_mu B) ->
