cast_sub/subtyping/AmberLocal.v
@@ -1,0 +1,177 @@
+Require Import Metalib.Metatheory.
+Require Import Program.Equality.
+Require Export Rules.
+Require Export Infra.
+Require Export AmberBase.
+Require Import Lia.
+
+Inductive WFC :  typ -> nat -> Prop :=
+| WC_nat: forall k,
+    WFC typ_nat k
+| WF_top: forall k,
+    WFC typ_top k
+| WF_fvar: forall X k,
+    WFC (typ_fvar X) k
+| WF_bvar: forall b k,
+    b < k ->
+    WFC (typ_bvar b) k
+| WF_arrow: forall A B k,
+    WFC A k ->
+    WFC B k ->
+    WFC (typ_arrow A B) k
+| WF_rec: forall A n,
+    WFC A (S n) ->
+    WFC (typ_mu A) n
+.
+
+#[global] Hint Constructors WFC : core.
+
+
+Fixpoint close_tt_rec (K : nat) (Z : atom) (T : typ) {struct T} : typ :=
+  match T with
+  | typ_nat         => typ_nat      
+  | typ_top         => typ_top              
+  | typ_bvar J      => typ_bvar J
+  | typ_fvar X      => if X == Z then typ_bvar K else typ_fvar X 
+  | typ_arrow T1 T2 => typ_arrow (close_tt_rec K Z T1) (close_tt_rec K Z T2)
+  | typ_mu T        => typ_mu (close_tt_rec (S K) Z T)
+  end.
+
+Definition close_tt T X := close_tt_rec 0 X T.
+
+Lemma close_wfc : forall A X,
+    WFC A 0 ->
+    WFC (close_tt A X) 1.
+Proof with auto.  
+  intros A.
+  unfold close_tt.
+  generalize 0.
+  induction A;intros;try solve [dependent destruction H;simpl in *;auto]...
+  -
+    simpl...
+    destruct (a==X)...
+Qed.
+
+
+Lemma open_wfc : forall A (X:atom),
+    WFC A 1 -> 
+    WFC (open_tt A X) 0.
+Proof with auto.  
+  intros A.
+  unfold open_tt.
+  generalize 0.
+  induction A;intros;try solve [dependent destruction H;simpl in *;auto]...
+  -
+    simpl...
+    destruct (n0==n)...
+    inversion H;subst. constructor. lia.
+Qed.
+
+Lemma WFC_add_one : forall A k,
+    WFC A k -> WFC A (S k).
+Proof with auto.
+  intros.
+  induction H...
+Qed.
+
+
+Lemma close_open_reverse_rec: forall T X,
+    (X \notin fv_tt T) -> forall k, T = close_tt_rec k X (open_tt_rec k (typ_fvar X) T).
+Proof with auto.
+  intros T.
+  induction T;intros;simpl in *;try solve [f_equal;auto]...
+  -   
+    destruct (k==n)...
+    simpl...
+    destruct (X==X)...
+    destruct n0...
+  -
+    destruct (a==X)...
+    apply notin_singleton_1 in H...
+    destruct H...
+Qed.
+
+Lemma close_open_reverse: forall T X,
+    (X \notin fv_tt T) ->  T = close_tt (open_tt T (typ_fvar X)) X.
+Proof with auto.
+  intros.
+  apply close_open_reverse_rec...
+Qed.
+
+Lemma close_type_wfc: forall A,
+    type A -> WFC A 0.
+Proof with auto.
+  intros.
+  induction H;intros...
+  constructor...
+  (* apply WFC_add_one. *)
+  pick fresh X.
+  specialize_x_and_L X L.
+  apply close_wfc with (X:=X) in H0.
+  rewrite <- close_open_reverse in H0...
+Qed.
+
+
+Fixpoint weight (T:typ) : nat :=
+  match T with
+  | typ_nat => 1
+  | typ_top => 1
+  | typ_fvar _ => 1
+  | typ_bvar _ => 1
+  | typ_arrow A B => 1 + weight A + weight B
+  | typ_mu A => 1 + weight A
+  end.
+
+Lemma open_tt_weight: forall T (X:atom),
+    weight (open_tt T X) = weight T.
+Proof with auto.  
+  intros. unfold open_tt. generalize 0.
+  induction T;intros;simpl in *;try solve [auto]...
+  -
+    destruct (n0==n)...
+Qed.
+
+
+Lemma type_wfc_close_aux: forall k A,
+  weight A <= k ->
+  WFC A 0 -> type A.
+Proof with auto.
+  induction k.
+  { intros. destruct A; simpl in H;lia. }
+  intros.
+  inversion H0;subst...
+  - exfalso. lia.
+  - simpl in H. 
+    apply IHk in H1;try lia...
+    apply IHk in H2;try lia...
+  - simpl in H.
+    apply type_mu with (L:={}).
+    intros.
+    apply IHk...
+    2:{ apply open_wfc... }
+    rewrite open_tt_weight...
+    lia.
+Qed.
+
+Lemma type_wfc_close: forall A,
+  WFC A 0 -> type A.
+Proof with auto.
+  intros.
+  apply type_wfc_close_aux with (k:=weight A)...
+Qed.
+
+
+
+
+
+Lemma type_open_tt_WFC :forall T X,
+    X \notin fv_tt T ->
+    type (open_tt T X) ->
+    WFC T 1.
+Proof with auto.
+  intros.
+  apply close_type_wfc in H0.
+  apply close_wfc with (X:=X) in H0...
+  rewrite <- close_open_reverse in H0...
+Qed.
+
